UniverseAbstractions/Lemmas/DerivedProductFunctors.lean
@@ -1,0 +1,183 @@
+import UniverseAbstractions.Axioms.Universes
+import UniverseAbstractions.Axioms.Universe.Functors
+import UniverseAbstractions.Axioms.Universe.Products
+import UniverseAbstractions.Lemmas.DerivedFunctors
+
+
+
+set_option autoBoundImplicitLocal false
+--set_option pp.universes true
+
+
+
+namespace HasFunctorialProducts
+
+  open HasEmbeddedProducts
+
+  variable {U : Universe} [HasEmbeddedFunctors U] [HasFunctorialProducts U]
+
+  def defFstFun [HasSubLinearFunOp U] (α β : U) : α ⊓ β ⟶[λ P => fst P] α :=
+  elimFun (HasSubLinearFunOp.constFunFun β α)
+  ◄ λ _ => by simp
+
+  def defSndFun [HasAffineFunOp    U] (α β : U) : α ⊓ β ⟶[λ P => snd P] β :=
+  elimFun (HasSubLinearFunOp.constFun α (HasLinearFunOp.idFun β))
+  ◄ λ _ => by simp
+
+  @[reducible] def fstFun [HasSubLinearFunOp U] (α β : U) : α ⊓ β ⟶ α := defFstFun α β
+  @[reducible] def sndFun [HasAffineFunOp    U] (α β : U) : α ⊓ β ⟶ β := defSndFun α β
+
+  def defDupIntroFun [HasNonLinearFunOp U] (α : U) : α ⟶[λ a => intro a a] α ⊓ α :=
+  HasNonLinearFunOp.dupFun (introFunFun α α)
+  ◄ λ _ => by simp
+
+  @[reducible] def dupIntroFun [HasNonLinearFunOp U] (α : U) : α ⟶ α ⊓ α := defDupIntroFun α
+
+  def defRevIntroFun [HasLinearFunOp U] (α : U) {β : U} (b : β) : α ⟶[λ a => intro a b] α ⊓ β :=
+  HasLinearFunOp.swapFun (introFunFun α β) b
+  ◄ λ _ => by simp
+
+  @[reducible] def revIntroFun [HasLinearFunOp U] (α : U) {β : U} (b : β) : α ⟶ α ⊓ β := defRevIntroFun α b
+
+  def defRevIntroFunFun [HasLinearFunOp U] (α β : U) : β ⟶[λ b => revIntroFun α b] (α ⟶ α ⊓ β) :=
+  HasLinearFunOp.swapFunFun (introFunFun α β)
+  ◄ λ _ => by simp [revIntroFun, defRevIntroFun]
+
+  @[reducible] def revIntroFunFun [HasLinearFunOp U] (α β : U) : β ⟶ α ⟶ α ⊓ β := defRevIntroFunFun α β
+
+  def defRevElimFun [HasLinearFunOp U] {α β γ : U} (F : β ⟶ α ⟶ γ) :
+    α ⊓ β ⟶[λ P => F (snd P) (fst P)] γ :=
+  elimFun (HasLinearFunOp.swapFunFun F)
+  ◄ λ _ => by simp
+
+  @[reducible] def revElimFun [HasLinearFunOp U] {α β γ : U} (F : β ⟶ α ⟶ γ) : α ⊓ β ⟶ γ := defRevElimFun F
+
+  def defRevElimFunFun [HasLinearFunOp U] (α β γ : U) : (β ⟶ α ⟶ γ) ⟶[λ F => revElimFun F] (α ⊓ β ⟶ γ) :=
+  elimFunFun α β γ ⊙ HasLinearFunOp.swapFunFunFun β α γ
+  ◄ λ _ => by simp [revElimFun, defRevElimFun]
+
+  @[reducible] def revElimFunFun [HasLinearFunOp U] (α β γ : U) : (β ⟶ α ⟶ γ) ⟶ (α ⊓ β ⟶ γ) := defRevElimFunFun α β γ
+
+  def invElim [HasLinearFunOp U] {α β γ : U} (F : α ⊓ β ⟶ γ) (a : α) (b : β) : γ := F (intro a b)
+
+  def defInvElimFun [HasLinearFunOp U] {α β γ : U} (F : α ⊓ β ⟶ γ) (a : α) : β ⟶[λ b => invElim F a b] γ :=
+  F ⊙ introFun a β
+  ◄ λ _ => by simp [invElim]
+
+  @[reducible] def invElimFun [HasLinearFunOp U] {α β γ : U} (F : α ⊓ β ⟶ γ) (a : α) : β ⟶ γ := defInvElimFun F a
+
+  def defInvElimFunFun [HasLinearFunOp U] {α β γ : U} (F : α ⊓ β ⟶ γ) : α ⟶[λ a => invElimFun F a] (β ⟶ γ) :=
+  HasLinearFunOp.revCompFunFun β F ⊙ introFunFun α β
+  ◄ λ _ => by simp [invElimFun, defInvElimFun]
+
+  @[reducible] def invElimFunFun [HasLinearFunOp U] {α β γ : U} (F : α ⊓ β ⟶ γ) : α ⟶ β ⟶ γ := defInvElimFunFun F
+
+  def defInvElimFunFunFun [HasLinearFunOp U] (α β γ : U) : (α ⊓ β ⟶ γ) ⟶[λ P => invElimFunFun P] (α ⟶ β ⟶ γ) :=
+  HasLinearFunOp.compFunFun (introFunFun α β) (β ⟶ γ) ⊙ HasLinearFunOp.revCompFunFunFun β (α ⊓ β) γ
+  ◄ λ _ => by simp [invElimFunFun, defInvElimFunFun]
+
+  @[reducible] def invElimFunFunFun [HasLinearFunOp U] (α β γ : U) : (α ⊓ β ⟶ γ) ⟶ (α ⟶ β ⟶ γ) :=
+  defInvElimFunFunFun α β γ
+
+  def defReplaceFstFun [HasLinearFunOp U] {α β : U} (F : α ⟶ β) (γ : U) :
+    α ⊓ γ ⟶[λ P => intro (F (fst P)) (snd P)] β ⊓ γ :=
+  elimFun (introFunFun β γ ⊙ F)
+  ◄ λ _ => by simp
+
+  @[reducible] def replaceFstFun [HasLinearFunOp U] {α β : U} (F : α ⟶ β) (γ : U) : α ⊓ γ ⟶ β ⊓ γ :=
+  defReplaceFstFun F γ
+
+  def defReplaceFstFunFun [HasLinearFunOp U] (α β γ : U) :
+    (α ⟶ β) ⟶[λ F => replaceFstFun F γ] (α ⊓ γ ⟶ β ⊓ γ) :=
+  elimFunFun α γ (β ⊓ γ) ⊙ HasLinearFunOp.revCompFunFun α (introFunFun β γ)
+  ◄ λ _ => by simp [replaceFstFun, defReplaceFstFun]
+
+  @[reducible] def replaceFstFunFun [HasLinearFunOp U] (α β γ : U) : (α ⟶ β) ⟶ (α ⊓ γ ⟶ β ⊓ γ) :=
+  defReplaceFstFunFun α β γ
+
+  def defReplaceSndFun [HasLinearFunOp U] {α β : U} (F : α ⟶ β) (γ : U) :
+    γ ⊓ α ⟶[λ P => intro (fst P) (F (snd P))] γ ⊓ β :=
+  revElimFun (revIntroFunFun γ β ⊙ F)
+  ◄ λ _ => by simp
+
+  @[reducible] def replaceSndFun [HasLinearFunOp U] {α β : U} (F : α ⟶ β) (γ : U) : γ ⊓ α ⟶ γ ⊓ β :=
+  defReplaceSndFun F γ
+
+  def defReplaceSndFunFun [HasLinearFunOp U] (α β γ : U) :
+    (α ⟶ β) ⟶[λ F => replaceSndFun F γ] (γ ⊓ α ⟶ γ ⊓ β) :=
+  revElimFunFun γ α (γ ⊓ β) ⊙ HasLinearFunOp.revCompFunFun α (revIntroFunFun γ β)
+  ◄ λ _ => by simp [replaceSndFun, defReplaceSndFun]
+
+  @[reducible] def replaceSndFunFun [HasLinearFunOp U] (α β γ : U) : (α ⟶ β) ⟶ (γ ⊓ α ⟶ γ ⊓ β) :=
+  defReplaceSndFunFun α β γ
+
+  def defCommFun [HasLinearFunOp U] (α β : U) : α ⊓ β ⟶[λ P => intro (snd P) (fst P)] β ⊓ α :=
+  elimFun (revIntroFunFun β α)
+  ◄ λ _ => by simp
+
+  @[reducible] def commFun [HasLinearFunOp U] (α β : U) : α ⊓ β ⟶ β ⊓ α := defCommFun α β
+
+  def intro₃LFunFun [HasLinearFunOp U] (α β γ : U) : α ⟶ β ⟶ γ ⟶ (α ⊓ β) ⊓ γ :=
+  HasLinearFunOp.revCompFunFun β (introFunFun (α ⊓ β) γ) ⊙ introFunFun α β
+  def intro₃RFunFun [HasLinearFunOp U] (α β γ : U) : α ⟶ β ⟶ γ ⟶ α ⊓ (β ⊓ γ) :=
+  invElimFunFunFun β γ (α ⊓ (β ⊓ γ)) ⊙ introFunFun α (β ⊓ γ)
+
+  def elim₃LFun                    {α β γ δ : U} (F : α ⟶ β ⟶ γ ⟶ δ) : (α ⊓ β) ⊓ γ ⟶ δ := elimFun (elimFun F)
+  def elim₃RFun [HasLinearFunOp U] {α β γ δ : U} (F : α ⟶ β ⟶ γ ⟶ δ) : α ⊓ (β ⊓ γ) ⟶ δ := elimFun (elimFunFun β γ δ ⊙ F)
+
+  def defAssocLRFun [HasLinearFunOp U] (α β γ : U) :
+    (α ⊓ β) ⊓ γ ⟶[λ P => intro (fst (fst P)) (intro (snd (fst P)) (snd P))] α ⊓ (β ⊓ γ) :=
+  elim₃LFun (intro₃RFunFun α β γ)
+  ◄ λ _ => by simp [elim₃LFun, intro₃RFunFun, invElimFunFun, defInvElimFunFun]
+
+  def defAssocRLFun [HasLinearFunOp U] (α β γ : U) :
+    α ⊓ (β ⊓ γ) ⟶[λ P => intro (intro (fst P) (fst (snd P))) (snd (snd P))] (α ⊓ β) ⊓ γ :=
+  elim₃RFun (intro₃LFunFun α β γ)
+  ◄ λ _ => by simp [elim₃RFun, intro₃LFunFun]
+
+  @[reducible] def assocLRFun [HasLinearFunOp U] (α β γ : U) : (α ⊓ β) ⊓ γ ⟶ α ⊓ (β ⊓ γ) := defAssocLRFun α β γ
+  @[reducible] def assocRLFun [HasLinearFunOp U] (α β γ : U) : α ⊓ (β ⊓ γ) ⟶ (α ⊓ β) ⊓ γ := defAssocRLFun α β γ
+
+  def defMergeFun [HasFullFunOp U] {α β γ : U} (F : α ⟶ β) (G : α ⟶ γ) :
+    α ⟶[λ a => intro (F a) (G a)] β ⊓ γ :=
+  HasFullFunOp.substFun F (revIntroFunFun β γ ⊙ G)
+  ◄ λ _ => by simp
+
+  @[reducible] def mergeFun [HasFullFunOp U] {α β γ : U} (F : α ⟶ β) (G : α ⟶ γ) : α ⟶ β ⊓ γ := defMergeFun F G
+
+  def defMergeFunFun [HasFullFunOp U] {α β : U} (F : α ⟶ β) (γ : U) :
+    (α ⟶ γ) ⟶[λ G => mergeFun F G] (α ⟶ β ⊓ γ) :=
+  HasFullFunOp.substFunFun F (β ⊓ γ) ⊙ HasLinearFunOp.revCompFunFun α (revIntroFunFun β γ)
+  ◄ λ _ => by simp [mergeFun, defMergeFun]
+
+  @[reducible] def mergeFunFun [HasFullFunOp U] {α β : U} (F : α ⟶ β) (γ : U) : (α ⟶ γ) ⟶ (α ⟶ β ⊓ γ) :=
+  defMergeFunFun F γ
+
+  def defMergeFunFunFun [HasFullFunOp U] (α β γ : U) : (α ⟶ β) ⟶[λ F => mergeFunFun F γ] ((α ⟶ γ) ⟶ (α ⟶ β ⊓ γ)) :=
+  HasLinearFunOp.compFunFun (HasLinearFunOp.revCompFunFun α (revIntroFunFun β γ)) (α ⟶ β ⊓ γ) ⊙
+  HasFullFunOp.substFunFunFun α β (β ⊓ γ)
+  ◄ λ _ => by simp [mergeFunFun, defMergeFunFun]
+
+  @[reducible] def mergeFunFunFun [HasFullFunOp U] (α β γ : U) : (α ⟶ β) ⟶ (α ⟶ γ) ⟶ (α ⟶ β ⊓ γ) :=
+  defMergeFunFunFun α β γ
+
+  def distr [HasAffineFunOp U] {α β γ : U} (F : α ⟶ β ⊓ γ) : (α ⟶ β) ⊓ (α ⟶ γ) :=
+  intro (fstFun β γ ⊙ F) (sndFun β γ ⊙ F) -- TODO: Rewrite using tactic, as a test
+
+  def defDistrFun [HasFullFunOp U] (α β γ : U) : (α ⟶ β ⊓ γ) ⟶[λ F => distr F] (α ⟶ β) ⊓ (α ⟶ γ) :=
+  mergeFun (HasLinearFunOp.revCompFunFun α (fstFun β γ)) (HasLinearFunOp.revCompFunFun α (sndFun β γ))
+  ◄ λ _ => by simp [distr]
+
+  @[reducible] def distrFun [HasFullFunOp U] (α β γ : U) : (α ⟶ β ⊓ γ) ⟶ (α ⟶ β) ⊓ (α ⟶ γ) := defDistrFun α β γ
+
+  def invDistrFun [HasFullFunOp U] {α β γ : U} (P : (α ⟶ β) ⊓ (α ⟶ γ)) : α ⟶ β ⊓ γ :=
+  mergeFun (fst P) (snd P)
+
+  def defInvDistrFunFun [HasFullFunOp U] (α β γ : U) : (α ⟶ β) ⊓ (α ⟶ γ) ⟶[λ P => invDistrFun P] (α ⟶ β ⊓ γ) :=
+  elimFun (mergeFunFunFun α β γ)
+  ◄ λ _ => by simp [invDistrFun]
+
+  @[reducible] def invDistrFunFun [HasFullFunOp U] (α β γ : U) : (α ⟶ β) ⊓ (α ⟶ γ) ⟶ (α ⟶ β ⊓ γ) :=
+  defInvDistrFunFun α β γ
+
+end HasFunctorialProducts
